code/experimental/P256/Hacl.Impl.P256.fst
@@ -23,6 +23,7 @@ open FStar.Math.Lemmas
 friend Hacl.Spec.P256.MontgomeryMultiplication
 open FStar.Mul
 
+
 inline_for_extraction noextract 
 val toDomain: value: felem -> result: felem ->  Stack unit 
   (requires fun h ->  as_nat h value < prime /\ live h value /\live h result /\ eq_or_disjoint value result)
@@ -128,7 +129,7 @@ let multByTwo a out =
 inline_for_extraction noextract 
 val multByThree: a: felem -> result: felem -> Stack unit 
   (requires fun h -> live h a /\ live h result /\ disjoint a result /\ as_nat h a < prime )
-  (ensures fun h0 _ h1 -> modifies (loc result) h0 h1 /\ as_nat h1 result < prime /\as_seq h1 result == mm_byThree_seq (as_seq h0 a))
+  (ensures fun h0 _ h1 -> modifies (loc result) h0 h1 /\ as_nat h1 result < prime)
 
 let multByThree a result = 
   multByTwo a result;
@@ -137,7 +138,7 @@ let multByThree a result =
 inline_for_extraction noextract 
 val multByFour: a: felem -> result: felem -> Stack unit 
   (requires fun h -> live h a /\ live h result /\ disjoint a result /\ as_nat h a < prime )
-  (ensures fun h0 _ h1 -> modifies (loc result) h0 h1 /\ as_nat h1 result < prime /\ as_seq h1 result == mm_byFour_seq (as_seq h0 a))
+  (ensures fun h0 _ h1 -> modifies (loc result) h0 h1 /\ as_nat h1 result < prime)
 
 let multByFour a result  = 
   multByTwo a result;
@@ -146,7 +147,7 @@ let multByFour a result  =
 inline_for_extraction noextract 
 val multByEight: a: felem -> result: felem -> Stack unit 
   (requires fun h -> live h a /\ live h result /\ disjoint a result /\ as_nat h a < prime )
-  (ensures fun h0 _ h1 -> modifies (loc result) h0 h1 /\ as_nat h1 result < prime /\ as_seq h1 result == mm_byEight_seq (as_seq h0 a))
+  (ensures fun h0 _ h1 -> modifies (loc result) h0 h1 /\ as_nat h1 result < prime)
 
 let multByEight a result  = 
   multByTwo a result;
@@ -156,7 +157,7 @@ let multByEight a result  =
 inline_for_extraction noextract 
 val multByMinusThree: a: felem -> result: felem -> Stack unit 
   (requires fun h -> live h a /\ live h result /\ disjoint a result /\ as_nat h a < prime )
-  (ensures fun h0 _ h1 -> modifies (loc result) h0 h1 /\ as_nat h1 result < prime /\ as_seq h1 result == mm_byMinusThree_seq (as_seq h0 a))
+  (ensures fun h0 _ h1 -> modifies (loc result) h0 h1 /\ as_nat h1 result < prime)
 
 let multByMinusThree a result  = 
   push_frame();
@@ -168,7 +169,7 @@ let multByMinusThree a result  =
 
 val isZero_uint64:  f: felem -> Stack uint64
   (requires fun h -> live h f /\ as_nat h f < prime)
-  (ensures fun h0 r h1 -> modifies0 h0 h1 /\ r == isZero_seq (as_seq h0 f))
+  (ensures fun h0 r h1 -> modifies0 h0 h1)
 
 let isZero_uint64 f = 
   let a0 = index f (size 0) in 
@@ -180,8 +181,8 @@ let isZero_uint64 f =
 
 val copy_point: p: point -> result: point -> Stack unit 
   (requires fun h -> live h p /\ live h result /\ disjoint p result) 
-  (ensures fun h0 _ h1 -> modifies (loc result) h0 h1 /\
-    as_seq h1 result == copy_point_seq (as_seq h0 p))
+  (ensures fun h0 _ h1 -> modifies (loc result) h0 h1 (* /\
+    as_seq h1 result == copy_point_seq (as_seq h0 p) *) )
 
 let copy_point p result = copy result p
  
@@ -203,8 +204,8 @@ val point_double_compute_s_m: p: point -> s: felem -> m: felem -> tempBuffer:lbu
      felem_seq_as_nat x_sequence < prime /\
      felem_seq_as_nat y_sequence < prime /\
      felem_seq_as_nat z_sequence < prime /\  
-  modifies (loc tempBuffer |+| loc s |+| loc m) h0 h1 /\ as_nat h1 s < prime  /\ as_nat h1 m < prime /\
-   (let (s_, m_) = point_double_compute_s_m_seq (as_seq h0 p) in as_seq h1 s == s_ /\ as_seq h1 m == m_))
+  modifies (loc tempBuffer |+| loc s |+| loc m) h0 h1 /\ as_nat h1 s < prime  /\ as_nat h1 m < prime 
+   (*(let (s_, m_) = point_double_compute_s_m_seq (as_seq h0 p) in as_seq h1 s == s_ /\ as_seq h1 m == m_) *) )
 
 
 let point_double_compute_s_m p s m tempBuffer =
@@ -228,10 +229,10 @@ let point_double_compute_s_m p s m tempBuffer =
     multByMinusThree zzzz minThreeZzzz;
     montgomery_square px xx;
     multByThree xx threeXx;
-    p256_add minThreeZzzz threeXx m;
-  let h1 = ST.get() in 
-  assert(let s_, m_ = point_double_compute_s_m_seq (as_seq h0 p) in Lib.Sequence.equal (s_) (as_seq h1 s)
-    /\ Lib.Sequence.equal m_ (as_seq h1 m))
+    p256_add minThreeZzzz threeXx m
+  (* let h1 = ST.get() in  *)
+  (* assert(let s_, m_ = point_double_compute_s_m_seq (as_seq h0 p) in Lib.Sequence.equal (s_) (as_seq h1 s) *)
+    (* /\ Lib.Sequence.equal m_ (as_seq h1 m)) *)
 
 
 inline_for_extraction noextract 
@@ -243,7 +244,7 @@ val point_double_compute_x3: x3: felem ->
     as_nat h s < prime /\ as_nat h m < prime 
   )
   (ensures fun h0 _ h1 -> modifies2 x3 tempBuffer h0 h1 /\
-    as_seq h1 x3 == point_double_compute_x3_seq (as_seq h0 s) (as_seq h0 m) /\ 
+    (* as_seq h1 x3 == point_double_compute_x3_seq (as_seq h0 s) (as_seq h0 m) /\  *)
     as_nat h1 x3 < prime
    )
 
@@ -264,7 +265,7 @@ val point_double_compute_y3: p_y: felem ->  y3: felem ->  x3: felem ->
     as_nat h p_y < prime)
     
   (ensures fun h0 _ h1 -> modifies2 y3 tempBuffer h0 h1 /\ 
-    as_seq h1 y3 == point_double_compute_y3_seq (as_seq h0 p_y) (as_seq h0 x3) (as_seq h0 s) (as_seq h0 m) /\
+    (* as_seq h1 y3 == point_double_compute_y3_seq (as_seq h0 p_y) (as_seq h0 x3) (as_seq h0 s) (as_seq h0 m) /\ *)
     as_nat h1 y3 < prime
    )
 
@@ -316,7 +317,7 @@ let point_double p result tempBuffer =
      concat3 (size 4) x3 (size 4) y3 (size 4) z3 result ; 
 
    let hend = ST.get() in 
-   assert(as_seq hend result == point_double_seq (as_seq h0 p));
+   (* assert(as_seq hend result == point_double_seq (as_seq h0 p)); *)
    assert(modifies1 tempBuffer h0 h5);
    assert(modifies2 tempBuffer result h0 hend)
 
@@ -324,8 +325,8 @@ let point_double p result tempBuffer =
 inline_for_extraction noextract 
 val copy_conditional: out: felem -> x: felem -> mask: uint64{uint_v mask = 0 \/ uint_v mask = pow2 64 - 1} -> Stack unit 
   (requires fun h -> live h out /\ live h x /\ as_nat h out < prime /\ as_nat h x < prime)
-  (ensures fun h0 _ h1 -> modifies1 out h0 h1 /\ as_nat h1 out < prime /\ 
-    as_seq h1 out == copy_conditional_seq (as_seq h0 out) (as_seq h0 x) mask 
+  (ensures fun h0 _ h1 -> modifies1 out h0 h1 /\ as_nat h1 out < prime (*/\ 
+    as_seq h1 out == copy_conditional_seq (as_seq h0 out) (as_seq h0 x) mask *)
   )
 
 let copy_conditional out x mask = 
@@ -347,8 +348,8 @@ let copy_conditional out x mask =
   upd out (size 2) temp_2;
   upd out (size 3) temp_3;
 
-    let h1 = ST.get() in 
-    assert(Lib.Sequence.equal (as_seq h1 out) (copy_conditional_seq (as_seq h0 out) (as_seq h0 x) mask))
+    let h1 = ST.get() in ()
+   (* assert(Lib.Sequence.equal (as_seq h1 out) (copy_conditional_seq (as_seq h0 out) (as_seq h0 x) mask)) *)
 
 
 val copy_point_conditional: x3_out: felem -> y3_out: felem -> z3_out: felem -> p: point -> maskPoint: point -> Stack unit
@@ -365,9 +366,9 @@ val copy_point_conditional: x3_out: felem -> y3_out: felem -> z3_out: felem -> p
   (ensures fun h0 _ h1 -> modifies (loc x3_out |+| loc y3_out |+| loc z3_out) h0 h1 /\ 
     as_nat h1 x3_out < prime /\
     as_nat h1 y3_out < prime /\
-    as_nat h1 z3_out < prime /\
+    as_nat h1 z3_out < prime (*/\
     (let xN, yN, zN = copy_point_conditional_seq (as_seq h0 x3_out) (as_seq h0 y3_out) (as_seq h0 z3_out) (as_seq h0 p) (as_seq h0 maskPoint) in 
-      xN == as_seq h1 x3_out /\ yN == as_seq h1 y3_out /\ zN == as_seq h1 z3_out)
+      xN == as_seq h1 x3_out /\ yN == as_seq h1 y3_out /\ zN == as_seq h1 z3_out) *)
     )
 
 let copy_point_conditional x3_out y3_out z3_out p maskPoint = 
@@ -387,7 +388,7 @@ let copy_point_conditional x3_out y3_out z3_out p maskPoint =
  
 val compare_felem: a: felem -> b: felem -> Stack uint64
   (requires fun h -> live h a /\ live h b /\ as_nat h a < prime /\ as_nat h b < prime ) 
-  (ensures fun h0 r h1 -> modifies0 h0 h1 /\ r == compare_felem_seq (as_seq h0 a) (as_seq h0 b)) 
+  (ensures fun h0 r h1 -> modifies0 h0 h1 (*/\ r == compare_felem_seq (as_seq h0 a) (as_seq h0 b))  *))
 
 let compare_felem a b = 
   let r0 = eq_mask a.(size 0) b.(size 0) in 
@@ -418,11 +419,11 @@ val move_from_jacobian_coordinates: u1: felem -> u2: felem -> s1: felem -> s2: f
     )
   (ensures fun h0 _ h1 -> 
     modifies (loc u1 |+| loc u2 |+| loc s1 |+| loc s2 |+| loc tempBuffer16) h0 h1 /\
-    as_nat h1 u1 < prime /\ as_nat h1 u2 < prime /\ as_nat h1 s1 < prime /\ as_nat h1 s2 < prime  /\
-    (
+    as_nat h1 u1 < prime /\ as_nat h1 u2 < prime /\ as_nat h1 s1 < prime /\ as_nat h1 s2 < prime  
+   (* /\(
       let u1_, u2_, s1_, s2_ = move_from_jacobian_coordinates_seq (as_seq h0 p) (as_seq h0 q) in 
       as_seq h1 u1 == u1_ /\ as_seq h1 u2 == u2_ /\ as_seq h1 s1 == s1_ /\ as_seq h1 s2 == s2_
-    )
+    ) *)
   )  
 
 let move_from_jacobian_coordinates u1 u2 s1 s2 p q tempBuffer = 
@@ -458,9 +459,9 @@ let move_from_jacobian_coordinates u1 u2 s1 s2 p q tempBuffer =
    montgomery_multiplication_buffer y2 z1Cube s2;
 
      let h3 = ST.get() in 
-      assert(modifies2 s1 s2 h2 h3);
-     assert(let u1_, u2_, s1_, s2_ = move_from_jacobian_coordinates_seq (as_seq h0 p) (as_seq h0 q) in 
-      as_seq h3 u1 == u1_ /\ as_seq h3 u2 == u2_ /\ as_seq h3 s1 == s1_ /\ as_seq h3 s2 == s2_)
+      assert(modifies2 s1 s2 h2 h3)
+     (*assert(let u1_, u2_, s1_, s2_ = move_from_jacobian_coordinates_seq (as_seq h0 p) (as_seq h0 q) in 
+      as_seq h3 u1 == u1_ /\ as_seq h3 u2 == u2_ /\ as_seq h3 s1 == s1_ /\ as_seq h3 s2 == s2_) *)
       
       
 inline_for_extraction noextract 
@@ -469,8 +470,8 @@ val compute_common_params_point_add: h: felem -> r: felem -> uh: felem -> hCube:
   Stack unit 
     (requires fun h0 -> live h0 h /\ live h0 r /\ live h0 uh /\ live h0 hCube /\ live h0 u1 /\ live h0 u2 /\ live h0 s1 /\ live h0 s2 /\ live h0 tempBuffer /\  LowStar.Monotonic.Buffer.all_disjoint [loc u1; loc u2; loc s1; loc s2; loc h; loc r; loc uh; loc hCube; loc tempBuffer] /\ 
   as_nat h0 u1 < prime /\ as_nat h0 u2 < prime /\ as_nat h0 s1 < prime /\ as_nat h0 s2 < prime)
-    (ensures fun h0 _ h1 ->  modifies (loc h |+| loc r |+| loc uh |+| loc hCube |+| loc tempBuffer) h0 h1 /\ as_nat h1 h < prime /\ as_nat h1 r < prime /\ as_nat h1 uh < prime /\ as_nat h1 hCube < prime /\
-      (let (hN, rN, uhN, hCubeN) = compute_common_params_point_add_seq (as_seq h0 u1) (as_seq h0 u2) (as_seq h0 s1) (as_seq h0 s2) in  as_seq h1 h == hN /\ as_seq h1 r == rN /\ as_seq h1 uh == uhN /\ as_seq h1 hCube == hCubeN)
+    (ensures fun h0 _ h1 ->  modifies (loc h |+| loc r |+| loc uh |+| loc hCube |+| loc tempBuffer) h0 h1 /\ as_nat h1 h < prime /\ as_nat h1 r < prime /\ as_nat h1 uh < prime /\ as_nat h1 hCube < prime (*/\
+      (let (hN, rN, uhN, hCubeN) = compute_common_params_point_add_seq (as_seq h0 u1) (as_seq h0 u2) (as_seq h0 s1) (as_seq h0 s2) in  as_seq h1 h == hN /\ as_seq h1 r == rN /\ as_seq h1 uh == uhN /\ as_seq h1 hCube == hCubeN) *)
     )
 
 
@@ -488,8 +489,9 @@ val computeX3_point_add: x3: felem -> hCube: felem -> uh: felem -> r: felem -> t
     LowStar.Monotonic.Buffer.all_disjoint [loc x3; loc hCube; loc uh; loc r; loc tempBuffer] /\
     as_nat h0 hCube < prime /\as_nat h0 uh < prime /\ as_nat h0 r < prime
   )
-  (ensures fun h0 _ h1 -> modifies2 x3 tempBuffer h0 h1 /\ as_nat h1 x3 < prime /\ 
-    as_seq h1 x3 == computeX3_point_add_seq (as_seq h0 hCube) (as_seq h0 uh) (as_seq h0 r) 
+  (ensures fun h0 _ h1 -> modifies2 x3 tempBuffer h0 h1 /\ as_nat h1 x3 < prime 
+  (*/\ 
+    as_seq h1 x3 == computeX3_point_add_seq (as_seq h0 hCube) (as_seq h0 uh) (as_seq h0 r)  *)
   )
 
 let computeX3_point_add x3 hCube uh r tempBuffer = 
@@ -508,8 +510,11 @@ val computeY3_point_add:y3: felem -> s1: felem -> hCube: felem -> uh: felem -> x
   Stack unit (requires fun h -> live h y3 /\ live h s1 /\ live h hCube /\ live h uh /\ live h x3_out /\ live h r /\ live h tempBuffer /\
     LowStar.Monotonic.Buffer.all_disjoint [loc y3; loc s1; loc hCube; loc uh; loc x3_out; loc r; loc tempBuffer] /\
     as_nat h s1 < prime /\ as_nat h hCube < prime /\ as_nat h uh < prime /\ as_nat h x3_out <prime /\ as_nat h r < prime)
-    (ensures fun h0 _ h1 -> modifies2 y3 tempBuffer h0 h1 /\ as_nat h1 y3 < prime /\ 
-    as_seq h1 y3 ==  computeY3_point_add_seq (as_seq h0 s1) (as_seq h0 hCube) (as_seq h0 uh) (as_seq h0 x3_out) (as_seq h0 r))
+    (ensures fun h0 _ h1 -> modifies2 y3 tempBuffer h0 h1 /\ as_nat h1 y3 < prime (*/\ 
+    as_seq h1 y3 ==  computeY3_point_add_seq (as_seq h0 s1) (as_seq h0 hCube) (as_seq h0 uh) (as_seq h0 x3_out) (as_seq h0 r)
+    *)
+    
+    )
     
 let computeY3_point_add y3 s1 hCube uh x3_out r tempBuffer = 
     let s1hCube = sub tempBuffer (size 0) (size 4) in 
@@ -526,8 +531,9 @@ val computeZ3_point_add: z3: felem ->  z1: felem -> z2: felem -> h: felem -> tem
   Stack unit (requires fun h0 -> live h0 z3 /\ live h0 z1 /\ live h0 z2 /\ live h0 h /\ live h0 tempBuffer /\ live h0 z3 /\
   LowStar.Monotonic.Buffer.all_disjoint [loc z1; loc z2; loc h; loc tempBuffer; loc z3] /\
   as_nat h0 z1 < prime /\ as_nat h0 z2 < prime /\ as_nat h0 h < prime)
-  (ensures fun h0 _ h1 -> modifies2 z3 tempBuffer h0 h1 /\ as_nat h1 z3 < prime /\ 
-    as_seq h1 z3 == computeZ3_point_add_seq (as_seq h0 z1) (as_seq h0 z2) (as_seq h0 h)
+  (ensures fun h0 _ h1 -> modifies2 z3 tempBuffer h0 h1 /\ as_nat h1 z3 < prime 
+  (*/\ 
+    as_seq h1 z3 == computeZ3_point_add_seq (as_seq h0 z1) (as_seq h0 z2) (as_seq h0 h) *)
   )  
 
 let computeZ3_point_add z3 z1 z2 h tempBuffer = 
@@ -541,7 +547,7 @@ val point_double_condition: u1: felem -> u2: felem -> s1: felem -> s2: felem ->z
     as_nat h u1 < prime /\ as_nat h u2 < prime /\ as_nat h s1 < prime /\ as_nat h s2 < prime /\
     as_nat h z1 < prime /\ as_nat h z2 < prime /\ 
     LowStar.Monotonic.Buffer.all_disjoint [loc u1; loc u2; loc s1; loc s2; loc z1; loc z2])
-  (ensures fun h0 r h1 -> modifies0 h0 h1 /\ r == point_double_condition_seq (as_seq h0 u1) (as_seq h0 u2) (as_seq h0 s1) (as_seq h0 s2) (as_seq h0 z1) (as_seq h0 z2))   
+  (ensures fun h0 r h1 -> modifies0 h0 h1 (*/\ r == point_double_condition_seq (as_seq h0 u1) (as_seq h0 u2) (as_seq h0 s1) (as_seq h0 s2) (as_seq h0 z1) (as_seq h0 z2) *) )   
 
 let point_double_condition u1 u2 s1 s2 z1 z2 = 
   let one = compare_felem u1 u2 in (* if equal -> 1111, else 000 *) (*1111*)
@@ -566,12 +572,16 @@ val point_add_if_second_branch_impl: result: point -> p: point -> q: point -> u1
     as_nat h0 (gsub p (size 4) (size 4)) < prime /\
     as_nat h0 (gsub q (size 8) (size 4)) < prime /\ 
     as_nat h0 (gsub q (size 0) (size 4)) < prime /\  
-    as_nat h0 (gsub q (size 4) (size 4)) < prime /\
+    as_nat h0 (gsub q (size 4) (size 4)) < prime (*/\
     (let u1_, u2_, s1_, s2_ = move_from_jacobian_coordinates_seq (as_seq h0 p) (as_seq h0 q) in 
     u1_ == (as_seq h0 u1) /\ u2_ == (as_seq h0 u2) /\ s1_ == (as_seq h0 s1) /\ s2_ == (as_seq h0 s2)) /\
-    (let h_, r_, uh_, hCube_ = compute_common_params_point_add_seq (as_seq h0 u1) (as_seq h0 u2) (as_seq h0 s1) (as_seq h0 s2) in h_ == (as_seq h0 h) /\ r_ == (as_seq h0 r) /\ uh_ == (as_seq h0 uh) /\ hCube_ == (as_seq h0 hCube)))
-  (ensures fun h0 _ h1 -> modifies2 tempBuffer28 result h0 h1 /\ 
-    as_seq h1 result == point_add_if_second_branch_seq (as_seq h0 p) (as_seq h0 q) (as_seq h0 u1) (as_seq h0 u2) (as_seq h0 s1) (as_seq h0 s2) (as_seq h0 r) (as_seq h0 h) (as_seq h0 uh) (as_seq h0 hCube))
+    (let h_, r_, uh_, hCube_ = compute_common_params_point_add_seq (as_seq h0 u1) (as_seq h0 u2) (as_seq h0 s1) (as_seq h0 s2) in h_ == (as_seq h0 h) /\ r_ == (as_seq h0 r) /\ uh_ == (as_seq h0 uh) /\ hCube_ == (as_seq h0 hCube)) *)
+    )
+  (ensures fun h0 _ h1 -> modifies2 tempBuffer28 result h0 h1 (*/\ 
+    as_seq h1 result == point_add_if_second_branch_seq (as_seq h0 p) (as_seq h0 q) (as_seq h0 u1) (as_seq h0 u2) (as_seq h0 s1) (as_seq h0 s2) (as_seq h0 r) (as_seq h0 h) (as_seq h0 uh) (as_seq h0 hCube)
+    *)
+    
+    )
 
 let point_add_if_second_branch_impl result p q u1 u2 s1 s2 r h uh hCube tempBuffer28 = 
     let h0 = ST.get() in 
@@ -606,8 +616,8 @@ let point_add_if_second_branch_impl result p q u1 u2 s1 s2 r h uh hCube tempBuff
   concat3 (size 4) x3_out (size 4) y3_out (size 4) z3_out result; 
     let h6 = ST.get() in 
     assert(modifies1 result h5 h6);
-    assert(modifies2 tempBuffer28 result h0 h6);
-    assert(Lib.Sequence.equal (as_seq h6 result) (point_add_if_second_branch_seq (as_seq h0 p) (as_seq h0 q) (as_seq h0 u1) (as_seq h0 u2) (as_seq h0 s1) (as_seq h0 s2) (as_seq h0 r) (as_seq h0 h) (as_seq h0 uh) (as_seq h0 hCube)))
+    assert(modifies2 tempBuffer28 result h0 h6) (*;
+    assert(Lib.Sequence.equal (as_seq h6 result) (point_add_if_second_branch_seq (as_seq h0 p) (as_seq h0 q) (as_seq h0 u1) (as_seq h0 u2) (as_seq h0 s1) (as_seq h0 s2) (as_seq h0 r) (as_seq h0 h) (as_seq h0 uh) (as_seq h0 hCube))) *)
     
  
 #reset-options "--z3rlimit 200"
@@ -647,8 +657,8 @@ let point_add p q result tempBuffer =
 	point_double p result tempBuffer;
 	let h0_2 = ST.get() in 
 	  assert(modifies2 tempBuffer result h0_1 h0_2);
-	  assert(modifies2 tempBuffer result h0 h0_2);
-	  assert(Lib.Sequence.equal (as_seq h0_2 result) (point_add_seq (as_seq h0 p) (as_seq h0 q)))
+	  assert(modifies2 tempBuffer result h0 h0_2)
+	 (* assert(Lib.Sequence.equal (as_seq h0_2 result) (point_add_seq (as_seq h0 p) (as_seq h0 q))) *)
      end	   
    else
      begin
@@ -662,10 +672,10 @@ let point_add p q result tempBuffer =
 	   assert(modifies2 tempBuffer result h1_2 h1_3)
      end; 
    let hend = ST.get() in   
-   assert(modifies2 tempBuffer result h0 hend);
-   assert(Lib.Sequence.equal (as_seq hend result) (point_add_seq (as_seq h0 p) (as_seq h0 q)))
+   assert(modifies2 tempBuffer result h0 hend)
+   (*assert(Lib.Sequence.equal (as_seq hend result) (point_add_seq (as_seq h0 p) (as_seq h0 q))) *)
 
-(* 4 minutes *)
+
 
 inline_for_extraction noextract 
 val uploadOneImpl: f: felem -> Stack unit
